RenameApart.v
@@ -1,7 +1,7 @@
 Require Import CSet Le.
 
 Require Import Plus Util Map.
-Require Import Env EnvTy IL Liveness Coherence Alpha Fresh.
+Require Import Env EnvTy IL Liveness Coherence Alpha Fresh Annotation.
 
 Set Implicit Arguments.
 
@@ -41,6 +41,11 @@ match s with
       (G'', stmtIf (rename_exp ϱ e) s1' s2')
    | stmtGoto l Y => (G, stmtGoto l (List.map (rename_exp ϱ) Y))
    | stmtReturn e => (G, stmtReturn (rename_exp ϱ e))
+   | stmtExtern x f Y s =>
+     let y := fresh G in
+     let ϱ' := ϱ[x <- y] in
+     let (G', s') := rename_apart' ϱ' (G ∪ {{y}}) s in
+       (G', stmtExtern y f (List.map (rename_exp ϱ) Y) s')
    | stmtLet Z s1 s2 =>
      let Y := fresh_list G (length Z) in
      let ϱZ := ϱ [ Z <-- Y ] in
@@ -58,6 +63,10 @@ match s with
      let ϱ' := rename_apart_rho ϱ s1 in rename_apart_rho ϱ' s2
    | stmtGoto l Y => ϱ
    | stmtReturn x => ϱ
+   | stmtExtern x f Y s =>
+     let y := fresh (freeVars s \ {{x}}) in
+     let ϱ' := ϱ[x <- y] in
+     rename_apart_rho ϱ' s
    | stmtLet Z s1 s2 =>
      let Y := fresh_list (freeVars s1) (length Z) in
      let ϱZ := ϱ [ Z <-- Y ]  in
@@ -69,8 +78,9 @@ Lemma rename_apart_incl ϱ G G' s
   : G ⊆ G' -> G ⊆ fst (rename_apart' ϱ G' s).
 Proof.
   general induction s; simpl; repeat let_pair_case_eq; simpl; subst; eauto.
-  eapply IHs. cset_tac. left; eauto.
-  eapply IHs2. eapply IHs1. cset_tac. left; eauto.
+  - eapply IHs. cset_tac. left; eauto.
+  - eapply IHs. cset_tac. left; eauto.
+  - eapply IHs2. eapply IHs1. cset_tac. left; eauto.
 Qed.
 
 Lemma rename_apart_incl_eq ϱ G G' s G''
@@ -86,9 +96,9 @@ Lemma rename_apart_notOccur G G' ϱ s
 Proof.
   general induction s; simpl; repeat let_pair_case_eq; simpl; eauto using notOccur; subst; eauto.
 
-  + econstructor; simpl in *.
-    - intro. eapply fresh_spec. eapply H, minus_incl; eauto.
-    - eapply notOccur_incl. Focus 2. eapply IHs. eapply Subset_refl.
+  - econstructor; simpl in *.
+    + intro. eapply fresh_spec. eapply H, minus_incl; eauto.
+    + eapply notOccur_incl. Focus 2. eapply IHs. eapply Subset_refl.
       hnf; intros. eapply lookup_set_spec in H1. destruct H1; dcr.
       lud. cset_tac; eauto. eapply union_2. eapply H0. eapply lookup_set_spec. intuition.
       eexists x0; cset_tac; intuition. intuition.
@@ -97,11 +107,11 @@ Proof.
       eapply lookup_set_spec in H1. destruct H1; dcr; eauto. lud.
       rewrite H5 in H2. exfalso. eapply fresh_spec; eauto.
       exists x0. cset_tac; intuition. intuition.
-    - eapply notOccur_freeVars.
+    + eapply notOccur_freeVars.
       cset_tac; intuition. eapply rename_exp_freeVars in H3.
       eapply H4. eapply lookup_set_incl; eauto; intuition. intuition.
 
-  + econstructor.
+  - econstructor.
     eapply Exp.notOccur_freeVars. cset_tac; intuition.
     eapply rename_exp_freeVars in H3; eauto.
     eapply H4. eapply lookup_set_spec; eauto. eapply lookup_set_spec in H3; eauto.
@@ -121,7 +131,7 @@ Proof.
     apply rename_apart_incl.
     simpl in *. eapply Subset_trans; eauto. eapply lookup_set_incl; eauto.
     cset_tac; intuition.
-  + econstructor. intros.
+  - econstructor. intros.
     edestruct map_get_4; eauto; dcr; subst.
     eapply Exp.notOccur_freeVars. cset_tac; intuition.
     eapply rename_exp_freeVars in H5; eauto.
@@ -130,14 +140,38 @@ Proof.
     destruct H5; dcr. eexists x0; intuition.
     eapply incl_list_union.
     eapply map_get_1; eauto. reflexivity. eauto.
-  + econstructor.
+  - econstructor.
     eapply Exp.notOccur_freeVars. cset_tac; intuition.
     eapply rename_exp_freeVars in H3; eauto.
-  + econstructor.
-    - cset_tac; intuition. rewrite H in H1.
+  - econstructor; eauto.
+    + intros.
+      edestruct map_get_4; eauto; dcr; subst.
+      eapply Exp.notOccur_freeVars. cset_tac; intuition.
+      eapply rename_exp_freeVars in H5; eauto.
+      eapply H6. eapply lookup_set_spec; eauto.
+      eapply lookup_set_spec in H5; eauto.
+      destruct H5; dcr. eexists x1; intuition.
+      eapply incl_right. eapply incl_list_union.
+      eapply map_get_1; eauto. reflexivity. eauto.
+    + intro. eapply fresh_spec. eapply H, minus_incl; eauto.
+    + eapply notOccur_incl.
+      Focus 2.
+      eapply IHs; try reflexivity.
+      hnf; intros. eapply lookup_set_spec in H1; eauto. destruct H1; dcr.
+      lud. cset_tac; eauto. eapply union_2. eapply H0.
+      eapply lookup_set_spec; eauto. intuition.
+      eexists x0; cset_tac; intuition. simpl.
+      eapply incl_left. cset_tac; intuition.
+      hnf; intros. cset_tac. left; eauto. intro.
+      eapply H3. eapply lookup_set_spec. intuition.
+      eapply lookup_set_spec in H1; eauto. destruct H1; dcr; eauto. lud.
+      rewrite H5 in H2. exfalso. eapply fresh_spec; eauto.
+      exists x0. cset_tac; intuition.
+  - econstructor.
+    + cset_tac; intuition. rewrite H in H1.
       eapply (not_in_empty a). rewrite <- (fresh_set_spec G' (length Z)).
       cset_tac; eauto.
-    - eapply notOccur_incl. Focus 2. eapply IHs1. reflexivity.
+    + eapply notOccur_incl. Focus 2. eapply IHs1. reflexivity.
       rewrite lookup_set_update_with_list_in_union_length.
       eapply incl_union_lr. simpl in *. eapply Subset_trans;try eassumption.
       eapply lookup_set_incl. intuition.  cset_tac; eauto. reflexivity. intuition.
@@ -151,10 +185,10 @@ Proof.
       eapply fresh_set_spec. cset_tac; eauto.
       rewrite fresh_list_length; eauto.
       eapply H3. eapply lookup_set_spec. intuition.
-      rewrite update_with_list_no_update in H5; eauto. eexists x.
+      erewrite update_with_list_no_update in H5; eauto. eexists x.
       split; eauto. cset_tac; eauto.
       eapply update_with_list_proper.
-    - eapply notOccur_incl. Focus 2. eapply IHs2. reflexivity.
+    + eapply notOccur_incl. Focus 2. eapply IHs2. reflexivity.
       eapply Subset_trans. Focus 2. eapply rename_apart_incl. reflexivity.
       eapply Subset_trans. Focus 2. eapply union_subset_1.
       simpl in H0. rewrite <- H0. eapply lookup_set_incl. intuition. cset_tac.
@@ -167,54 +201,350 @@ Qed.
 
 Opaque to_list.
 
+Fixpoint ssa_ann (s:stmt) (G:set var) : ann (set var * set var) :=
+  match s with
+    | stmtExp x e s =>
+      let an := ssa_ann s (G ∪ {{x}}) in
+      ann1 (G,snd (getAnn an)) an
+    | stmtIf e s t =>
+      let ans := ssa_ann s G in
+      let ant := ssa_ann t G in
+      ann2 (G, snd (getAnn ans) ∪ snd (getAnn ant)) ans ant
+    | stmtReturn e =>
+      ann0 (G, G)
+    | stmtGoto f Y =>
+      ann0 (G, G)
+    | stmtExtern x f Y s =>
+      let an := ssa_ann s (G ∪ {{x}}) in
+      ann1 (G,snd (getAnn an)) an
+    | stmtLet Z s t =>
+      let ans := ssa_ann s (G ∪ of_list Z) in
+      let ant := ssa_ann t G in
+      ann2 (G, snd (getAnn ans) ∪ snd (getAnn ant)) ans ant
+  end.
+
+Instance pe_trans X `{OrderedType X} : Transitive (@pe _ _).
+Proof.
+  hnf; intros ? ? ? B C.
+  eapply prod_Equivalence_obligation_3; eauto using Equal_ST.
+Qed.
+
+Instance getAnn_ann_R_morphism A (R:A->A->Prop)
+: Proper (ann_R R ==> R) (getAnn).
+Proof.
+  unfold Proper, respectful; intros.
+  inv H; simpl; eauto.
+Qed.
+
+Instance ssa_ann_morph
+: Proper (eq ==> Equal ==> ann_R (@pe _ _ )) ssa_ann.
+Proof.
+  unfold Proper, respectful; intros. subst.
+  general induction y; simpl; eauto using ann_R.
+  - econstructor. rewrite H0 at 1. rewrite IHy. reflexivity.
+    rewrite H0; reflexivity.
+    eapply IHy. rewrite H0; reflexivity.
+  - econstructor; eauto.
+    rewrite H0 at 1. rewrite IHy1, IHy2; eauto. reflexivity.
+  - econstructor; rewrite H0; reflexivity.
+  - econstructor; rewrite H0; reflexivity.
+  - econstructor. rewrite H0 at 1. rewrite IHy. reflexivity.
+    rewrite H0; reflexivity.
+    eapply IHy. rewrite H0; reflexivity.
+  - econstructor; eauto.
+    rewrite H0 at 1.
+    rewrite IHy1, IHy2; eauto. reflexivity.
+    rewrite H0; reflexivity.
+    eapply IHy1. rewrite H0. reflexivity.
+Qed.
+
+Lemma ssa_ann_decomp s G
+: pe (getAnn (ssa_ann s G)) (G, snd (getAnn (ssa_ann s G))).
+Proof.
+  destruct s; simpl; try reflexivity.
+Qed.
+
+Lemma ssa_ann_app_incl s G G' G''
+: G' ∪ G'' [=] G
+  -> snd (getAnn (ssa_ann s G)) [=] G' ++ snd (getAnn (ssa_ann s G'')).
+Proof.
+  intros. general induction s; simpl.
+  - rewrite IHs. reflexivity. rewrite <- H. rewrite union_assoc. reflexivity.
+  - rewrite (IHs1 _ _ _ H) at 1.
+    erewrite (IHs2 _ _ {}); [|rewrite union_comm, empty_neutral_union; reflexivity].
+    symmetry.
+    erewrite (IHs2 _ _ {}); [|rewrite union_comm, empty_neutral_union; reflexivity].
+    (* rewrite (IHs1 _ _ _ H) at 1. *)
+    rewrite <- H.
+    clear_all; cset_tac; intuition.
+  - rewrite H. reflexivity.
+  - rewrite H. reflexivity.
+  - rewrite IHs. reflexivity. rewrite <- H. rewrite union_assoc. reflexivity.
+  - erewrite (IHs2 _ _ {}); [|rewrite union_comm, empty_neutral_union; reflexivity].
+    erewrite (IHs1 _ _ {}); [|rewrite union_comm, empty_neutral_union; reflexivity].
+    symmetry.
+    erewrite (IHs2 _ _ {}); [|rewrite union_comm, empty_neutral_union; reflexivity].
+    erewrite (IHs1 _ _ {}); [|rewrite union_comm, empty_neutral_union; reflexivity].
+    rewrite <- H. clear_all; cset_tac; intuition.
+Qed.
+
+Lemma rename_apart_fst_incl ϱ s G
+: G ⊆ fst (rename_apart' ϱ G s).
+Proof.
+  intros.
+  general induction s; simpl; repeat let_pair_case_eq; simpl; subst; eauto; try reflexivity; try now (rewrite <- IHs; cset_tac; intuition).
+  - rewrite <- IHs2, <- IHs1; reflexivity.
+  - rewrite <- IHs2, <- IHs1. cset_tac; intuition.
+Qed.
+
+Lemma rename_apart_fst_incl_app ϱ s G
+: fst (rename_apart' ϱ G s) [=] fst (rename_apart' ϱ G s) ∪ G.
+Proof.
+  pose proof (@rename_apart_fst_incl ϱ s G).
+  cset_tac; intuition.
+Qed.
+
+Lemma ssa_ann_rename_apart s G ϱ
+: snd (getAnn (ssa_ann (snd (rename_apart' ϱ G s)) G)) [=] fst (rename_apart' ϱ G s).
+Proof.
+  general induction s; simpl; repeat let_pair_case_eq; simpl; subst; eauto; try reflexivity.
+  - rewrite IHs1 at 1. rewrite <- IHs2. rewrite <- ssa_ann_app_incl. reflexivity.
+    rewrite rename_apart_fst_incl_app. cset_tac; intuition.
+  - rewrite <- IHs2. rewrite IHs1 at 1.
+    rewrite <- ssa_ann_app_incl. reflexivity.
+    symmetry.
+    rewrite rename_apart_fst_incl_app.
+    cset_tac; intuition.
+Qed.
+
+
+
+Lemma ssa_ann_rename_apart' s G G' ϱ
+: G ⊆ G'
+  -> snd (getAnn (ssa_ann (snd (rename_apart' ϱ G' s)) G)) [=] fst (rename_apart' ϱ G' s) \ (G' \ G).
+Proof.
+  general induction s; simpl; repeat let_pair_case_eq; simpl; subst; eauto; try reflexivity.
+  - rewrite IHs at 1. cset_tac; intuition.
+    eapply H0; intros. intuition.
+    eapply fresh_spec. instantiate (1:=G'). rewrite <- H6. eauto.
+    rewrite H. reflexivity.
+  - rewrite IHs1. rewrite IHs2.
+    rewrite rename_apart_fst_incl_app at 3.
+    cset_tac; intuition.
+    eapply rename_apart_fst_incl; eauto.
+    decide ( a \In fst (rename_apart' ϱ G' s1)); intuition.
+    rewrite H. eapply rename_apart_fst_incl; eauto. eauto.
+  - cset_tac; intuition. decide (a ∈ G); intuition.
+  - cset_tac; intuition. decide (a ∈ G); intuition.
+  - rewrite IHs; try reflexivity. cset_tac; intuition.
+    eapply H0; intros; intuition.
+    eapply fresh_spec. instantiate (1:=G'). rewrite <- H6. eauto.
+    rewrite H. reflexivity.
+  - rewrite IHs2. rewrite IHs1.
+    cset_tac; intuition.
+    + eapply rename_apart_fst_incl; eauto.
+    + eapply H1; intros. destruct H2; eauto.
+      exploit (fresh_list_spec G' (length Z) a); dcr.
+      exploit H6; eauto. cset_tac; intuition. cset_tac; intuition.
+    + eapply H1; intros.
+      eapply rename_apart_fst_incl; eauto. cset_tac; intuition. eauto.
+    + decide ( a \In
+                 fst
+                 (rename_apart' (ϱ [Z <-- fresh_list G' (length Z)])
+                                (G' ++ of_list (fresh_list G' (length Z))) s1)); intuition.
+    + rewrite H. reflexivity.
+    + rewrite <- rename_apart_fst_incl. rewrite H. eapply incl_left.
+Qed.
+
+Instance ann_R_trans A R `{Transitive A R} : Transitive (ann_R R).
+Proof.
+  hnf; intros ? ? ? B C.
+  general induction B; inv C; econstructor; eauto.
+Qed.
+
+Instance ann_R_ann1_pe_morphism X `{OrderedType X}
+: Proper (@pe X _ ==> ann_R (@pe X _) ==> ann_R (@pe X _)) (@ann1 _).
+Proof.
+  unfold Proper, respectful; intros.
+  econstructor; eauto.
+Qed.
+
+Instance pminus_morphism
+: Proper (Equal ==> (@pe _ _) ==> (@pe _ _) ) pminus.
+Proof.
+  unfold Proper, respectful; intros.
+  inv H0; simpl; econstructor. rewrite H1, <- H. reflexivity.
+  rewrite H2, H. reflexivity.
+Qed.
+
+Instance mapAnn_pminus_morphism G'
+  : Proper (ann_R (@pe _ _) ==> ann_R (@pe _ _)) (mapAnn (pminus G')).
+Proof.
+  unfold Proper, respectful; intros.
+  general induction H; simpl.
+  - econstructor; eauto.
+    + rewrite H. reflexivity.
+  - econstructor; eauto.
+    + rewrite H. reflexivity.
+  - econstructor; eauto.
+    + rewrite H. reflexivity.
+Qed.
+
+Lemma ann_R_pe_notOccur G G' s
+:  notOccur G' s
+   -> G \ G' [=] G
+   -> ann_R (@pe var _)
+           (ssa_ann s G)
+                     (mapAnn (pminus G') (ssa_ann s (G ∪ G'))).
+Proof.
+  intros. general induction H; simpl; try now (econstructor; reflexivity).
+  - assert ((G ++ G') ++ {x; {}} [=] (G ++ {{ x }}) ++ G'). {
+      cset_tac; intuition.
+    }
+    econstructor.
+    + rewrite H3. rewrite IHnotOccur.
+      rewrite getAnn_mapAnn. unfold pminus.
+      let_pair_case_eq; simpl; eauto.
+      econstructor; try reflexivity.
+      revert H2; clear_all; cset_tac; intuition.
+      eapply H2 in H; intuition.
+      rewrite <- H2.
+      revert H; clear_all; cset_tac; intuition.
+      eapply H; cset_tac.
+    + rewrite H3.
+      eapply IHnotOccur.
+      rewrite <- H2. revert H; clear_all; cset_tac; intuition.
+      eapply H. cset_tac.
+  - econstructor; eauto.
+    rewrite IHnotOccur1, IHnotOccur2; eauto.
+    repeat rewrite getAnn_mapAnn.
+    unfold pminus.
+    repeat let_pair_case_eq; simpl; eauto.
+    econstructor; try reflexivity.
+    rewrite <- H2. clear_all; cset_tac; intuition.
+    rewrite minus_dist_union. reflexivity.
+  - econstructor. econstructor; rewrite <- H0; clear_all; cset_tac; intuition.
+  - econstructor. econstructor; rewrite <- H0; clear_all; cset_tac; intuition.
+  - assert ((G ++ G') ++ {x; {}} [=] (G ++ {{ x }}) ++ G'). {
+      cset_tac; intuition.
+    }
+    econstructor.
+    + rewrite H3. rewrite IHnotOccur.
+      rewrite getAnn_mapAnn. unfold pminus.
+      let_pair_case_eq; simpl.
+      econstructor; try reflexivity.
+      rewrite <- H2; clear_all; cset_tac; intuition.
+      rewrite <- H2; revert H0; clear_all; cset_tac; intuition.
+      eapply H0; cset_tac.
+    + rewrite H3.
+      eapply IHnotOccur.
+      rewrite <- H2; revert H0; clear_all; cset_tac; intuition.
+      eapply H0; cset_tac.
+  - assert ((G ++ G') ++ of_list Z [=] (G ++ of_list Z) ++ G'). {
+      cset_tac; intuition.
+    }
+    econstructor; eauto.
+    + rewrite H3. rewrite IHnotOccur1.
+      rewrite getAnn_mapAnn. unfold pminus.
+      let_pair_case_eq; simpl.
+      econstructor. rewrite <- H2; clear_all; cset_tac; intuition.
+      rewrite IHnotOccur2, getAnn_mapAnn.
+      unfold pminus. let_pair_case_eq; simpl.
+      rewrite minus_dist_union. reflexivity.
+      eauto.
+      rewrite <- H2. revert H; clear_all; cset_tac; intuition; eauto.
+    + rewrite H3.
+      eapply IHnotOccur1.
+      rewrite <- H2. revert H; clear_all; cset_tac; intuition; eauto.
+Qed.
+
+
 Lemma rename_apart_ssa' (s:stmt) ϱ G
   : lookup_set ϱ (freeVars s) ⊆ G
-  -> ssa G (snd (rename_apart' ϱ G s)) (fst (rename_apart' ϱ G s)).
+  -> ssa (snd (rename_apart' ϱ G s)) (ssa_ann (snd (rename_apart' ϱ G s)) G).
 Proof.
-  general induction s; simpl; repeat let_pair_case_eq.
-  + subst. econstructor. eapply fresh_spec. simpl in H.
-    rewrite rename_exp_freeVars. eapply Subset_trans; eauto.
-    eapply lookup_set_incl. intuition. eapply union_subset_2. intuition.
-    eapply IHs. simpl in *. hnf; intros. eapply lookup_set_spec in H0; decompose records.
-    lud. rewrite H3. cset_tac. right; eauto.
-    rewrite union_comm. eapply incl_right. rewrite H3. eapply H.
-    eapply lookup_set_spec; eauto. eexists x0. split; eauto.
-    eapply union_2. eapply in_in_minus; eauto. cset_tac. intuition.
-
-  + subst s0 s4. simpl in H. simpl. rename s3 into Gs2. rename s into Gs1.
+  general induction s; simpl; repeat let_pair_case_eq; simpl.
+  - subst. econstructor; eauto using fresh_spec, ssa_ann_decomp.
+    + simpl in H.
+      rewrite rename_exp_freeVars; eauto. etransitivity; eauto.
+      eapply lookup_set_incl; eauto. intuition.
+    + eapply IHs. simpl in *.
+      hnf; intros. eapply lookup_set_spec in H0; eauto; dcr.
+      lud.
+      * rewrite H3. cset_tac. right; eauto.
+      * rewrite union_comm. eapply incl_right. rewrite H3. eapply H.
+        eapply lookup_set_spec; eauto. eexists x0. split; eauto.
+        eapply union_2. eapply in_in_minus; eauto. cset_tac.
+  - subst s0 s4. simpl in H. simpl. rename s3 into Gs2. rename s into Gs1.
     eapply ssaIf with (Ds := Gs1) (Dt := (Gs2 \ (Gs1 \ G))).
-    - rewrite <- H. rewrite Exp.rename_exp_freeVars; eauto.
+    + rewrite <- H. rewrite Exp.rename_exp_freeVars; eauto.
       eapply lookup_set_incl; eauto. eapply incl_right.
-    - eapply minus_incl_meet_special. subst; eapply rename_apart_incl. reflexivity.
+    + eapply minus_incl_meet_special. subst; eapply rename_apart_incl. reflexivity.
       subst. eapply rename_apart_incl; reflexivity.
-    - eapply minus_incl_special. subst. eapply rename_apart_incl. reflexivity.
-    - subst. eapply IHs1. eapply Subset_trans; eauto. eapply lookup_set_incl. intuition.
+    + rewrite minus_incl_special. subst.
+      * rewrite <- ssa_ann_rename_apart.
+        rewrite ssa_ann_app_incl; try reflexivity.
+        rewrite <- ssa_ann_rename_apart.
+        rewrite ssa_ann_rename_apart.
+        rewrite rename_apart_fst_incl_app at 2. reflexivity.
+      * subst. eapply rename_apart_incl. reflexivity.
+    + subst. eapply IHs1. etransitivity; eauto. eapply lookup_set_incl; eauto.
       eapply Subset_trans; [| eapply union_subset_1]. eapply union_subset_1.
-    - assert (G [=] (G \ (Gs1 \ G))). eapply minus_minus_eq.
-    rewrite H0 at 1. assert (Gs2 \ (Gs1 \ G) [=] (Gs2 \ (Gs1 \ G)) \ (Gs1 \ G)).
-    eapply minus_idem. rewrite H3.
-    eapply ssa_minus.
-    eapply notOccur_incl; try eapply rename_apart_notOccur with (G:=Gs1 \ G).
-    eapply Subset_trans. rewrite minus_idem. reflexivity. eapply incl_minus_lr.
-    reflexivity. eapply Subset_trans; eauto. eapply lookup_set_incl. intuition.
-    eapply Subset_trans; [| eapply union_subset_1]. eapply union_subset_2.
-    eapply incl_minus.
-    subst. eapply Subset_trans. Focus 2. eapply rename_apart_incl. reflexivity.
-    rewrite <- H. eapply lookup_set_incl. intuition. cset_tac; eauto.
-    assert (G [=] Gs1 \ (Gs1 \ G)). eapply minus_minus_id. subst. eapply rename_apart_incl. reflexivity.
-    rewrite H4 at 1. eapply ssa_minus.
-    eapply notOccur_incl; try eapply rename_apart_notOccur with (G:=Gs1 \ G). subst.
-    eapply Subset_trans. rewrite minus_idem. reflexivity. eapply incl_minus_lr.
-    reflexivity. eapply Subset_trans; eauto. eapply lookup_set_incl. intuition.
-    eapply Subset_trans; [| eapply union_subset_1]. eapply union_subset_2.
-    eapply incl_minus.
-    subst. eapply Subset_trans. Focus 2. eapply rename_apart_incl. reflexivity.
-    rewrite <- H. eapply lookup_set_incl. intuition. cset_tac; eauto.
-    subst. eapply IHs2. eapply Subset_trans; eauto using rename_apart_incl.
-    eapply lookup_set_incl. intuition.
-    eapply Subset_trans; [| eapply union_subset_1]. eapply union_subset_2.
+    + {
+        assert (G [=] (G \ (Gs1 \ G))) by eapply minus_minus_eq.
+        assert (Gs2 \ (Gs1 \ G) [=] (Gs2 \ (Gs1 \ G)) \ (Gs1 \ G))
+          by eapply minus_idem.
+        rewrite H0.
+        eapply ssa_minus. instantiate (1:=Gs1\G).
+        -  eapply notOccur_incl; try eapply rename_apart_notOccur with (G:=Gs1 \ G).
+          + eapply Subset_trans.
+            * rewrite minus_idem. reflexivity.
+            * eapply incl_minus_lr; try reflexivity.
+              eapply Subset_trans; eauto. eapply lookup_set_incl; eauto.
+              eapply Subset_trans; [| eapply union_subset_1]. eapply union_subset_2.
+          + eapply incl_minus.
+          + eapply Subset_trans.
+            * eapply Subset_trans; eauto. eapply lookup_set_incl; eauto.
+              eapply Subset_trans; [| eapply union_subset_1]. eapply union_subset_2.
+            * subst. eapply rename_apart_incl. reflexivity.
+        - eapply IHs2.
+          + eapply Subset_trans.
+            * eapply Subset_trans; eauto. eapply lookup_set_incl; eauto.
+              eapply Subset_trans; [| eapply union_subset_1]. eapply union_subset_2.
+            * subst. eapply rename_apart_incl. reflexivity.
+        -
+          intros. rewrite <- H0.
+          assert (G [=] (Gs1 \ (Gs1 \ G))). {
+          pose proof (@rename_apart_fst_incl ϱ s1 G). rewrite H1 in H4.
+          revert H4; clear_all; cset_tac; intuition.
+          decide (a ∈ G); eauto. exfalso. eauto.
+          }
+          assert (Gs1 [=] ((Gs1 \ (Gs1 \ G)) ++ (Gs1 \ G))). {
+          pose proof (@rename_apart_fst_incl ϱ s1 G). rewrite H1 in H5.
+          revert H4; clear_all; cset_tac; intuition.
+          decide (a ∈ G); intuition.
+          }
+          rewrite H4 at 1. rewrite H5 at 6. eapply ann_R_pe_notOccur.
+          eapply notOccur_incl; try eapply rename_apart_notOccur with (G:=Gs1 \ G).
+          + eapply Subset_trans.
+            * rewrite minus_idem. reflexivity.
+            * eapply incl_minus_lr; try reflexivity.
+              eapply Subset_trans; eauto. eapply lookup_set_incl; eauto.
+              eapply Subset_trans; [| eapply union_subset_1]. eapply union_subset_2.
+          + eapply incl_minus.
+          + eapply Subset_trans.
+            * eapply Subset_trans; eauto. eapply lookup_set_incl; eauto.
+              eapply Subset_trans; [| eapply union_subset_1]. eapply union_subset_2.
+            * subst. eapply rename_apart_incl. reflexivity.
+          + rewrite <- minus_idem. reflexivity.
+      }
+    + rewrite ssa_ann_decomp. rewrite ssa_ann_rename_apart.
+      subst; reflexivity.
+    + rewrite ssa_ann_decomp. rewrite <- H2.
+      rewrite ssa_ann_rename_apart'. reflexivity.
+      subst. eapply rename_apart_fst_incl.
 
-  + econstructor. simpl in H.
+  - econstructor. simpl in H.
     rewrite <- H.
     unfold list_union. rewrite lookup_set_list_union.
     instantiate (1:={}).
@@ -224,38 +554,106 @@ Proof.
     rewrite <- Exp.rename_exp_freeVars; eauto; reflexivity.
     hnf; intros. rewrite map_spec; eauto. cset_tac; intuition.
     destruct H0; cset_tac; eauto. reflexivity.
-  + econstructor. simpl in H. rewrite <- H.
+  - econstructor. simpl in H. rewrite <- H.
     rewrite Exp.rename_exp_freeVars; eauto.
     eapply lookup_set_incl; eauto.
     reflexivity. reflexivity.
+  - subst. econstructor; eauto using fresh_spec, ssa_ann_decomp.
+    + simpl in H.
+      assert  (lookup_set ϱ
+        (list_union (List.map Exp.freeVars Y)) [<=]G).
+      rewrite <- H.
+      eapply lookup_set_incl; eauto. eapply incl_right.
+      rewrite <- H0.
+      unfold list_union. rewrite lookup_set_list_union.
+      instantiate (1:={}).
+      eapply fold_left_subset_morphism; try reflexivity.
+      repeat rewrite map_map.
+      eapply map_ext_get; intros.
+      rewrite <- Exp.rename_exp_freeVars; eauto; reflexivity.
+      hnf; intros. rewrite map_spec; eauto. cset_tac; intuition.
+      destruct H1; cset_tac; eauto.
+    + eapply IHs. simpl in *.
+      hnf; intros. eapply lookup_set_spec in H0; eauto; dcr.
+      lud.
+      * rewrite H3. cset_tac. right; eauto.
+      * rewrite union_comm. eapply incl_right. rewrite H3. eapply H.
+        eapply lookup_set_spec; eauto. eexists x0. split; eauto.
+        eapply union_2. eapply in_in_minus; eauto. cset_tac.
 
-  + simpl. subst s0 s4. simpl in H. simpl. rename s3 into Gs2. rename s into Gs1.
+  - simpl. subst s0 s4. simpl in H. simpl. rename s3 into Gs2. rename s into Gs1.
     eapply ssaLet with (Ds:=Gs1) (Dt:=Gs2 \ (Gs1 \ G)).
-    - eapply fresh_set_spec.
-    - eapply  minus_incl_meet_special; eauto using rename_apart_incl_eq, incl_refl.
+    + eapply fresh_set_spec.
+    + eapply  minus_incl_meet_special; eauto using rename_apart_incl_eq, incl_refl.
       subst. eapply rename_apart_incl. eapply incl_left.
       subst. eapply rename_apart_incl. eapply Subset_refl.
-    - eapply minus_incl_special. subst. eapply rename_apart_incl. reflexivity.
-    - subst. rewrite union_comm. eapply IHs1.
-      rewrite lookup_set_update_with_list_in_union_length.
+    + rewrite ssa_ann_rename_apart; try reflexivity.
+      rewrite H1.
+      rewrite ssa_ann_rename_apart'. rewrite H2. reflexivity.
+      subst Gs1.
+      rewrite <- rename_apart_fst_incl. eapply incl_left.
+    + eapply IHs1.
+      rewrite lookup_set_update_with_list_in_union_length; eauto.
       eapply incl_union_lr; eauto. rewrite <- H.
-      eapply lookup_set_incl; eauto. intuition.
-      cset_tac; auto. intuition.
+      eapply lookup_set_incl; eauto. intuition. reflexivity.
       rewrite fresh_list_length; eauto.
-    - assert (G [=] (Gs1 \ (Gs1 \ G))). eapply minus_minus_id. subst. eapply rename_apart_incl.
-      eapply union_subset_1.
-      rewrite H0 at 1. eapply ssa_minus.
-      eapply notOccur_incl; try eapply rename_apart_notOccur with (G:=Gs1 \ G).
-      eapply Subset_trans. rewrite minus_idem. reflexivity. eapply incl_minus_lr.
-      reflexivity. eapply Subset_trans; eauto. eapply lookup_set_incl. intuition.
-      eapply Subset_trans; [| eapply union_subset_2]. reflexivity.
-      eapply incl_minus.
-      subst. eapply Subset_trans. Focus 2. eapply rename_apart_incl. reflexivity.
-      eapply Subset_trans;[|eapply union_subset_1].
-      rewrite <- H. eapply lookup_set_incl. intuition. cset_tac; eauto.
-      subst. eapply IHs2. eapply rename_apart_incl.
-      eapply Subset_trans; [| eapply union_subset_1]. eapply Subset_trans; eauto.
-      eapply lookup_set_incl. intuition. eapply union_subset_2.
+    + rewrite ssa_ann_decomp.
+      econstructor. rewrite union_comm. reflexivity.
+      rewrite ssa_ann_rename_apart. subst; reflexivity.
+    +  {
+        assert (G [=] (G \ (Gs1 \ G))) by eapply minus_minus_eq.
+        assert (Gs2 \ (Gs1 \ G) [=] (Gs2 \ (Gs1 \ G)) \ (Gs1 \ G))
+          by eapply minus_idem.
+        rewrite H0.
+        eapply ssa_minus. instantiate (1:=Gs1\G).
+        -  eapply notOccur_incl; try eapply rename_apart_notOccur with (G:=Gs1 \ G).
+          + eapply Subset_trans.
+            * rewrite minus_idem. reflexivity.
+            * eapply incl_minus_lr; try reflexivity.
+              eapply Subset_trans; eauto. eapply lookup_set_incl; eauto.
+              eapply incl_right.
+          + eapply incl_minus.
+          + eapply Subset_trans.
+            * eapply Subset_trans; eauto. eapply lookup_set_incl; eauto.
+              eapply incl_right.
+            * subst. eapply rename_apart_incl. eapply incl_left.
+        - eapply IHs2.
+          + eapply Subset_trans.
+            * eapply Subset_trans; eauto. eapply lookup_set_incl; eauto.
+              eapply incl_right.
+            * subst. eapply rename_apart_incl. eapply incl_left.
+        -
+          intros. rewrite <- H0.
+          assert (G [=] (Gs1 \ (Gs1 \ G))). {
+            assert (G ⊆ Gs1). rewrite <- H1.
+            rewrite <- rename_apart_fst_incl. eapply incl_left.
+            revert H4; clear_all; cset_tac; intuition.
+            decide (a ∈ G); eauto. exfalso. eauto.
+          }
+          assert (Gs1 [=] ((Gs1 \ (Gs1 \ G)) ++ (Gs1 \ G))). {
+            assert (G ⊆ Gs1). rewrite <- H1.
+            rewrite <- rename_apart_fst_incl. eapply incl_left.
+            revert H5; clear_all; cset_tac; intuition.
+            decide (a ∈ G); intuition.
+          }
+          rewrite H4 at 1. rewrite H5 at 6. eapply ann_R_pe_notOccur.
+          eapply notOccur_incl; try eapply rename_apart_notOccur with (G:=Gs1 \ G).
+          + eapply Subset_trans.
+            * rewrite minus_idem. reflexivity.
+            * eapply incl_minus_lr; try reflexivity.
+              eapply Subset_trans; eauto. eapply lookup_set_incl; eauto.
+              eapply incl_right.
+          + eapply incl_minus.
+          + eapply Subset_trans.
+            * eapply Subset_trans; eauto. eapply lookup_set_incl; eauto.
+              eapply incl_right.
+            * subst. eapply rename_apart_incl. eapply incl_left.
+          + rewrite <- minus_idem. reflexivity.
+      }
+    + rewrite ssa_ann_decomp. econstructor. reflexivity.
+      rewrite ssa_ann_rename_apart'. rewrite H2. reflexivity.
+      rewrite <- H1. rewrite <- rename_apart_fst_incl.
+      eapply incl_left.
 Qed.
 
 Lemma rename_apart_alpha' G ϱ ϱ' s
@@ -265,43 +663,59 @@ Lemma rename_apart_alpha' G ϱ ϱ' s
 Proof.
   general induction s; simpl; repeat let_pair_case_eq; subst; simpl in * |- *; eauto using alpha.
 
-  + econstructor. eapply alpha_exp_sym. eapply alpha_exp_rename_injective.
+  - econstructor. eapply alpha_exp_sym. eapply alpha_exp_rename_injective.
     eapply inverse_on_incl; eauto. cset_tac; eauto.
     eapply IHs.
-    - rewrite lookup_set_update_in_union.
+    + rewrite lookup_set_update_in_union.
       eapply incl_union_lr; try reflexivity. rewrite <- H.
       eapply lookup_set_incl. intuition. cset_tac; eauto. intuition.
-    - eapply inverse_on_update_inverse. intuition.
+    + eapply inverse_on_update_inverse. intuition.
       eapply inverse_on_incl; eauto. cset_tac; eauto.
       assert (lookup_set ϱ (freeVars s \ {{x}}) ⊆
                          lookup_set ϱ (freeVars s \ {{x}} ∪ Exp.freeVars e)).
       eapply lookup_set_incl. intuition. cset_tac; eauto.
       intro. eapply H1 in H2. eapply H in H2.
       eapply fresh_spec in H2. eauto.
-  + econstructor; eauto.
-    - eapply alpha_exp_sym. eapply Exp.alpha_exp_rename_injective.
+  - econstructor; eauto.
+    + eapply alpha_exp_sym. eapply Exp.alpha_exp_rename_injective.
       eapply inverse_on_incl; eauto. eapply incl_right.
-    - eapply IHs1.
+    + eapply IHs1.
       * eapply Subset_trans; eauto. eapply lookup_set_incl; [intuition|].
         rewrite union_assoc, union_comm. eapply incl_right.
       * eapply inverse_on_incl; eauto. rewrite union_assoc, union_comm. eapply incl_right.
-    - eapply IHs2; eauto.
+    + eapply IHs2; eauto.
       * eapply Subset_trans; eauto using rename_apart_incl. eapply lookup_set_incl; [intuition|].
         rewrite union_comm at 1. rewrite <- union_assoc. eapply incl_right.
       * eapply inverse_on_incl; eauto.
         rewrite union_comm at 1. rewrite <- union_assoc. eapply incl_right.
-  + econstructor. rewrite map_length; eauto.
+  - econstructor. rewrite map_length; eauto.
     intros. edestruct map_get_4; eauto; dcr; get_functional; subst.
     eapply alpha_exp_sym. eapply Exp.alpha_exp_rename_injective.
     eapply inverse_on_incl; eauto. eapply incl_list_union; try reflexivity.
     eapply map_get_1; eauto.
 
-  + econstructor; eauto. eapply alpha_exp_sym.
+  - econstructor; eauto. eapply alpha_exp_sym.
     eapply Exp.alpha_exp_rename_injective.
     eapply inverse_on_incl; eauto. reflexivity.
 
-  + econstructor. eapply fresh_list_length.
-    - eapply IHs1.
+  - econstructor.
+    + rewrite map_length; eauto.
+    + intros. edestruct map_get_4; eauto; dcr; get_functional; subst.
+      eapply alpha_exp_sym. eapply Exp.alpha_exp_rename_injective.
+      eapply inverse_on_incl; eauto. etransitivity; [| eapply incl_right].
+      eapply  incl_list_union; try reflexivity.
+      eapply map_get_1; eauto.
+    + eapply IHs; eauto.
+      * rewrite lookup_set_update_in_union.
+        eapply incl_union_lr; try reflexivity. rewrite <- H.
+        eapply lookup_set_incl. intuition. cset_tac; eauto. intuition.
+      * eapply inverse_on_update_inverse. intuition.
+        eapply inverse_on_incl; eauto. cset_tac; eauto.
+        rewrite lookup_set_incl; [ | eauto | eapply incl_left; eauto].
+        erewrite H.
+        eapply fresh_spec.
+  - econstructor. eapply fresh_list_length.
+    + eapply IHs1.
       * rewrite lookup_set_update_with_list_in_union_length.
         eapply incl_union_lr. rewrite <- H.
         eapply lookup_set_incl; intuition. reflexivity.
@@ -318,7 +732,7 @@ Proof.
         eexists x0. cset_tac; intuition.
         eapply (not_in_empty x).
         eapply fresh_list_spec. cset_tac; eauto. intuition.
-    - eapply IHs2.
+    + eapply IHs2.
       * eapply rename_apart_incl. eapply Subset_trans; [| eapply  union_subset_1].
         eapply Subset_trans; eauto. eapply lookup_set_incl;[intuition| eapply incl_right].
       * eapply inverse_on_incl; eauto. eapply incl_right.
@@ -329,9 +743,8 @@ Qed.
 Definition rename_apart s := snd (rename_apart' id (freeVars s) s).
 
 Lemma rename_apart_ssa (s:stmt)
-  : ssa (freeVars s) (rename_apart s) (fst (rename_apart' id (freeVars s) s)).
-Proof.
-  eapply rename_apart_ssa'. eapply lookup_set_on_id. eapply Subset_refl.
+  : ssa (rename_apart s) (ssa_ann (snd (rename_apart' id (freeVars s) s)) (freeVars s)).
+  eapply rename_apart_ssa'. eapply lookup_set_on_id. reflexivity.
 Qed.
 
 Lemma rename_apart_alpha s
